src/lang/Event.v
@@ -169,6 +169,12 @@ Module MachineEvent.
   | syscall (e: Event.t)
   | abort
   .
+
+  Definition is_abort (e: t): bool :=
+    match e with
+    | abort => true
+    | _ => false
+    end.
 End MachineEvent.
 
 
